Nonce allocation primitive.

primitives.v
@@ -1,11 +1,13 @@
 From mathcomp Require Import ssreflect.
 From stdpp Require Import gmap.
-From iris.algebra Require Import agree auth gmap.
+From iris.algebra Require Import agree auth gset gmap.
 From iris.base_logic.lib Require Import invariants.
 From iris.heap_lang Require Import notation proofmode.
 From crypto Require Import term crypto1.
 
-Definition mknonce : val := (λ: <>, ref #()).
+Definition mknonce : val := λ: <>,
+  let: "n" := ref #() in
+  (#2, "n").
 
 Definition eq_term : val := (rec: "eq" "x" "y" :=
   if: (Fst "x" = #0) && (Fst "y" = #0) then
@@ -42,6 +44,52 @@ Definition res_ctx : iProp Σ :=
 
 Global Instance persistent_res_ctx : Persistent res_ctx.
 Proof. apply _. Qed.
+
+Lemma twp_mknonce E rs :
+  ↑resN ⊆ E →
+  res_ctx -∗
+  wf_readers rs -∗
+  WP mknonce #()%V @ E
+     [{v, ∃ l, ⌜v = val_of_term (TNonce l)⌝
+               ∗ nonceT l rs}].
+Proof.
+move=> HE; iIntros "#? #wf_rs"; rewrite /mknonce.
+wp_pures; wp_alloc l as "Hl"; iApply fupd_twp.
+iInv resN as (RM1) "[Hown >wf_RM1]" "Hclose".
+iMod (later_own with "Hown") as (a) "[Hown Ha]".
+case: a=> [aa af]; rewrite auth_equivI /=.
+iDestruct "Ha" as "[Ha >Haf]"; iRewrite -"Haf" in "Hown".
+rewrite option_equivI; case: aa=> [[q a]|]; last by iMod "Ha" as "[]".
+rewrite prod_equivI /=; iDestruct "Ha" as "[> <- #Ha]".
+iPoseProof (own_valid with "Hown") as "#Hvalid".
+rewrite auth_validI /=.
+iDestruct "Hvalid" as "(_&Hvalid)".
+iDestruct "Hvalid" as (RR) "(e & _ & Hvalid)".
+iRewrite "e" in "Hown"; iRewrite "e" in "Ha"; iClear "e"; clear a af.
+rewrite -[Auth _ _]/(● RR) agree_equivI.
+iDestruct (to_resR_uninjI with "Hvalid") as (RM2) "e".
+iRewrite -"e" in "Hown"; iRewrite -"e" in "Ha".
+rewrite to_resR_equivI.
+iAssert (▷ (dom (gset loc) RM1 ≡ dom (gset loc) RM2))%I as "> %e".
+  by iModIntro; iRewrite "Ha".
+iAssert (⌜l ∉ dom (gset loc) RM2⌝)%I as "%Hfresh".
+  rewrite -e elem_of_dom; iIntros "%contra".
+  case: contra=> v RM_l; rewrite big_sepM_delete //.
+  iDestruct "wf_RM1" as "[[Hl' _] _]".
+  by iPoseProof (mapsto_valid_2 with "Hl Hl'") as "%".
+iMod (own_update _ _ (_ ⋅ ◯ {[l := to_agree (RNonce rs)]}) with "Hown")
+    as "[Hown ?]".
+  apply auth_update_alloc, alloc_singleton_local_update; last done.
+  by rewrite -not_elem_of_dom dom_fmap.
+iAssert (▷ res_inv)%I with "[Hl wf_RM1 Hown]" as "Hinv".
+  iModIntro. iRewrite -"Ha" in "Hown".
+  iExists (<[l:=RNonce rs]> RM1).
+  rewrite -fmap_insert; iFrame.
+  rewrite big_sepM_insert /=; first by iFrame.
+  by apply/not_elem_of_dom; rewrite e.
+iMod ("Hclose" with "Hinv") as "_".
+by iModIntro; wp_pures; eauto.
+Qed.
 
 Lemma twp_eq_term t1 t2 :
   ⊢ WP (eq_term (val_of_term t1) (val_of_term t2))
